RiscvDialect/InstructionSelection/BitVecProofExamples.lean
@@ -1,0 +1,29 @@
+open BitVec
+
+
+theorem test (a b : Bool) :
+  (a || b) = (b || a) := by ac_nf -- :)
+
+
+instance : Std.Commutative (fun a b : Bool => a == b) :=
+  ⟨fun a b =>
+  match a, b with
+  | true, true   => rfl
+  | true, false  => rfl
+  | false, true  => rfl
+  | false, false => rfl
+⟩
+
+
+
+#check  Std.Commutative
+
+
+  --⟨fun a b => by decide⟩
+
+
+#synth Std.Associative (· || ·) -- succeeds :)
+#synth Std.Commutative (· || ·) -- succeeds :)
+
+#synth Std.Associative (· == ·) -- fails :(
+#synth Std.Commutative (· == ·) -- fails :(
